Large commit

Backend/PythonAdapter.c
@@ -1,0 +1,109 @@
+#include <Python.h>
+#include <stdbool.h>
+
+typedef struct binary_tree_node_s {
+    int data;
+    struct binary_tree_node_s *left, *right;
+} BTNode;
+
+typedef struct opt {
+    bool safe;
+    BTNode* ptr;
+} Opt;
+
+#define None ((Opt){false, NULL})
+#define Some(x) ((Opt){true, x})
+
+
+Opt treeToC(PyObject*);
+void printTree(BTNode*);
+Opt proc();
+
+// Assume that PyObject is non-null.
+Opt treeToC (PyObject* value) {
+    if (value == NULL) {
+        return None;
+    }
+    if (Py_Is(value, Py_None)) {
+        return Some(NULL);
+    }
+    PyObject* data = PyObject_GetAttrString(value, "data");
+    if (!data || !PyLong_Check(data)) {
+        fprintf(stderr, "Invalid datum\n");
+        return None;
+    }
+    PyObject* left = PyObject_GetAttrString(value, "left");
+    PyObject* right = PyObject_GetAttrString(value, "right");
+    BTNode* result = malloc(sizeof(BTNode));
+    Opt ol = treeToC(left);
+    Opt or = treeToC(right);
+    if (!ol.safe) return None;
+    if (!or.safe) return None;
+    *result = (BTNode){PyLong_AsLong(data), ol.ptr, or.ptr};
+    Py_XDECREF(data);
+    Py_XDECREF(left);
+    Py_XDECREF(right);
+    return Some(result);
+}
+
+void printTree (BTNode* node) {
+    if (node == NULL) { printf("*"); return; }
+    printf("%d; ( ", node->data);
+    printTree(node->left);
+    printf(" ); ( ");
+    printTree(node->right);
+    printf(" )");
+}
+
+Opt proc() {
+    printf("Entering proc\n");
+    Py_Initialize();
+
+    PyObject* pModule1 = PyImport_Import(PyUnicode_FromString("sys"));
+    // PyObject res1 = PyRun_SimpleString("'Hello World'");
+
+    PyRun_SimpleString("import sys; print(sys.argv[0]); sys.path.append('./Backend')");
+    PyObject* pName = PyUnicode_FromString("script");
+    /* Error checking of pName left out */
+
+    PyObject* pModule = PyImport_Import(pName);
+    Py_DECREF(pName);
+
+    if (pModule == NULL) {
+        PyErr_Print();
+        printf("RET1\n");
+        return None;
+    }
+
+    PyObject* pFunc = PyObject_GetAttrString(pModule, "greet");
+    /* pFunc is a new reference */
+    if (!pFunc || !PyCallable_Check(pFunc)) {
+        if (PyErr_Occurred()) PyErr_Print();
+
+        Py_XDECREF(pFunc);
+        Py_DECREF(pModule);
+        Py_Finalize();
+
+        printf("RET2\n");
+        return None;
+    }
+
+    PyObject* pValue = PyObject_CallObject(pFunc, NULL);
+    if (pValue == NULL) {
+        fprintf(stderr, "Call failed\n");
+        printf("RET3\n");
+        return None;
+    }
+
+    Opt o = treeToC (pValue);
+    if (!o.safe) return None;
+    BTNode* node = o.ptr;
+    printTree(node);
+
+    printf("RET4\n");
+    return Some(node);
+}
+
+int hw() { return 1; }
+Opt hw2() { return None; }
+
