Backend/WithForLoops.lean
@@ -1,4 +1,3 @@
-import Backend.PythonAdapter
 import Lean
 
 open Lean
@@ -34,6 +33,7 @@ inductive Expr :=
 
 inductive Stmt :=
   | assign : Name -> Expr -> Stmt
+  | forLoop : List Stmt -> Stmt
 
 -- Consider functions to have a canonical form with one return only.
 structure FunDef :=
@@ -47,13 +47,31 @@ def Program := List FunDef
 
 end Py
 
+
+namespace PyExample
 def tN : String -> Name := (Name.str .anonymous ·)
 
 #check (.app (.var $ tN "l") $ .cons (.var $ tN "a") $ .cons (.var $ tN "b") $ .nil : Py.Shape)
+end PyExample
+
+def Tensor (l : Py.Shape) := { ℓ : Py.Shape // l = ℓ }
+namespace Tensor
+def mk : Tensor l := ⟨l, by rfl⟩
+def of (l : Py.Shape) : Tensor l := ⟨l, by rfl⟩
+end Tensor
+
+
+def isPrimOp (n : Name) : Bool :=
+  match n with
+  | .str .anonymous s =>
+    s == "tensorAddPrimOp"
+  | _ => false
 
 open Elab Command Term Meta
 
 namespace ElabPy
+
+#check Lean.Parser.Term.doSeq
 mutual
 partial def expr (e : Py.Expr) : CommandElabM (TSyntax `term) := do
   match e with
@@ -65,6 +83,9 @@ partial def expr (e : Py.Expr) : CommandElabM (TSyntax `term) := do
   | .var v => return mkIdent v
   | .add left right => `(($(<- expr left) + $(<- expr right)))
   | .matmul left right => `(($(<- expr left) @ $(<- expr right)))
+  | .call (.var n) args =>
+    if isPrimOp n then `($(<- fncall (.var n) args) ($(mkIdent `primOpResolve)))
+    else fncall (.var n) args
   | .call fn args => fncall fn args
 
 partial def fncall (fn : Py.Expr) (args : List Py.Expr) : CommandElabM (TSyntax `term) := do
@@ -73,15 +94,13 @@ partial def fncall (fn : Py.Expr) (args : List Py.Expr) : CommandElabM (TSyntax 
   | x::xs => `(($(<- fncall fn xs) $(<- expr x)))
 end
 
-def stmt (s : List Py.Stmt) (r : Py.Expr) : CommandElabM (TSyntax `term) := do
+def stmt (s : List Py.Stmt) (r : Py.Expr) : CommandElabM (TSyntax `Lean.Parser.Term.doSeq) := do
   match s with
   | [] => expr r
   | (.assign s ex)::xs =>`(
     let $(mkIdent s) := $(<- expr ex)
     $(<- stmt xs r)
   )
-
-def Tensor (l : Py.Shape) := { ℓ : Py.Shape // l = ℓ }
 
 def unAnnot : Py.Shape -> CommandElabM (TSyntax `term) := λ s => do
   match s with
@@ -102,14 +121,15 @@ def typ : Py.Typ -> CommandElabM (TSyntax `term) := λ t => do
   | .int => return mkIdent `Int
   | .float => return mkIdent `Float
   | .list t => `($(mkIdent `List) $(<- typ t))
-  | .tensor annot => `($(mkIdent `ElabPy.Tensor) $(<- unAnnot annot))
+  | .tensor annot => `($(mkIdent `Tensor) $(<- unAnnot annot))
 
 def func : Py.FunDef -> CommandElabM (TSyntax `command) :=
   λ ⟨n, p, b, r, rt⟩ => do
   let params := if p.length > 0 then p.toArray.map Prod.fst |>.map mkIdent else #[mkIdent `_]
 
-  `(def $(mkIdent n) : $(<- type (p.map Prod.snd) rt) := λ $(params)* =>
-    $(<- stmt b r))
+  let s := <- stmt b r
+  `(def $(mkIdent n) : $(<- type (p.map Prod.snd) rt) := λ $(params)* => Id.run do
+    $(s))
   where
     type (ps : List Py.Typ) (rt : Py.Typ) : CommandElabM (TSyntax `term) := do
       if ps.length == 0 then
@@ -134,9 +154,14 @@ syntax (name := pyFuncCmd) "#pyFunc" term : command
     liftTermElabM $ Tactic.TryThis.addSuggestion cmd.raw {suggestion := .tsyntax cmd}
   | _ => throwUnsupportedSyntax
 
-
+/-
+def exa(a : int, b : int) -> int:
+  x = a
+  y = x + 1
+  return x
+-/
 def exampleFunction : Py.FunDef := {
-  name := `qual
+  name := `exa
   params := [
     (`a, .int),
     (`b, .int)
@@ -149,6 +174,10 @@ def exampleFunction : Py.FunDef := {
   rettyp := .int
 }
 
+/-
+def tensorAddN(a : Tensor (l), b : Tensor (l)) -> Tensor (l):
+  return a + b
+-/
 def tensorAdd : Py.FunDef := {
   name := `tensorAddN
   params := [
@@ -160,8 +189,60 @@ def tensorAdd : Py.FunDef := {
   rettyp := .tensor (.var `l)
 }
 
+def tensorAddAltered : Py.FunDef := {
+  name := `tensorAddAltered2
+  params := [
+    (`a, .tensor (.var `l)),
+    (`b, .tensor (.var `l))
+  ]
+  body := []
+  retval := .call (.var `tensorAddPrimOp) [(.var `a), (.var `b)]
+  rettyp := .tensor (.var `l)
+}
 
-def tensorAddN :
-    ElabPy.Tensor (Py.Shape.var l) ->
-      ElabPy.Tensor (Py.Shape.var l) -> ElabPy.Tensor (Py.Shape.var l) :=
+instance : HAdd (Tensor (Py.Shape.var l)) (Tensor (Py.Shape.var l)) (Tensor (Py.Shape.var l)) where
+  hAdd _ _ := Tensor.mk
+
+-- class DecidablyTrue (p : Prop) := proof : p
+
+def AddRel (l : List Py.Shape) : Type := Unit
+
+-- instance [DecidablyTrue (AddRel a b)] : HAdd (Tensor a) (Tensor b) (Tensor a) where
+--   hAdd _ _ := Tensor.mk
+
+
+def tensorAddN : Tensor (Py.Shape.var l) -> Tensor (Py.Shape.var a) -> Tensor (Py.Shape.var l) :=
   λ a b => (a + b)
+
+class PrimOpD (r : List Py.Shape -> Type) :=
+  primOpResolve {l : List Py.Shape} : Option (r l)
+open PrimOpD
+
+def tensorAddPrimOp (t : Tensor a) (t' : Tensor b) (r : AddRel [a, b]) : Tensor a := sorry
+
+instance : PrimOpD AddRel where
+  primOpResolve := .none
+
+open Tactic
+
+elab "my_search" : tactic => do
+  Lean.Elab.Tactic.withMainContext do
+    let goal ← Lean.Elab.Tactic.getMainGoal
+    let goalDecl ← goal.getDecl
+    let goalType := goalDecl.type
+    dbg_trace f!"goal type: {goalType}"
+  -- let goals <- getGoals
+  -- if goals.isEmpty then return
+  -- try
+  --   evalTactic (← `(tactic| exact rfl))
+  -- catch _ =>
+  --   evalTactic (← `(tactic| apply Nat.add_comm; exact rfl))
+
+example : AddRel [(Py.Shape.var l), (Py.Shape.var l)] := by
+  my_search
+
+#pyFunc tensorAddAltered
+
+-- def tensorAddAltered2 :
+--     Tensor (Py.Shape.var l) -> Tensor (Py.Shape.var l) -> Tensor (Py.Shape.var l) := λ a b =>
+--   ((tensorAddPrimOp b) a)
