Backend/Demo.lean
@@ -1,0 +1,67 @@
+import Backend.DemoBase
+
+/-
+def exa(a : int, b : int) -> int:
+  x = a
+  y = x + 1
+  return x
+-/
+def exampleFunction : Py.FunDef := {
+  name := `exa
+  params := [
+    (`a, .float),
+    (`b, .float)
+  ]
+  body := [
+    .assign `x $ .var `a,
+    .assign `y $ .add (.var `x) (.int 1)
+  ]
+  retval := .var `x
+  rettyp := .int
+}
+
+/-
+def tensorAddN(a : Tensor (l), b : Tensor (l)) -> Tensor (l):
+  return a + b
+-/
+def tensorAdd : Py.FunDef := {
+  name := `tensorAddN
+  params := [
+    (`a, .tensor (.var `l)),
+    (`b, .tensor (.var `l))
+  ]
+  body := []
+  retval := .add (.var `a) (.var `b)
+  rettyp := .tensor (.var `l)
+}
+
+def tensorAddAltered : Py.FunDef := {
+  name := `tensorAddAlteration
+  params := [
+    (`a, .tensor (.var `l)),
+    (`b, .tensor (.var `l))
+  ]
+  body := []
+  retval := .call (.var `tensorAddPrimOp) [(.var `a), (.var `b)]
+  rettyp := .tensor (.var `l)
+}
+
+/-
+def tensorMatMul(
+  a : Tensor ([2] + [3, 4]),
+  b : Tensor ([2] + [4, 5])
+) -> Tensor ([2] + [3, 5]):
+  return a @ b
+-/
+def tensorMatMulAltered : Py.FunDef := {
+  name := `tensorMatMulAlteration
+  params := [
+    (`a, .tensor ((2 ::: ∅) ++ (3 ::: 4 ::: ∅))),
+    (`b, .tensor ((2 ::: ∅) ++ (4 ::: 5 ::: ∅)))
+  ]
+  body := []
+  retval := .call (.var `tensorMatMulPrimOp) [(.var `a), (.var `b)]
+  rettyp := .tensor ((2 ::: ∅) ++ (3 ::: 5 ::: ∅))
+}
+
+#pyFunc tensorMatMulAltered
