Backend/PythonAdapter.lean
@@ -1,0 +1,78 @@
+import Alloy.C
+
+
+open scoped Alloy.C
+
+alloy c include <lean/lean.h>
+alloy c include "stdio.h" "stdbool.h"
+
+alloy c section
+
+typedef struct binary_tree_node_s {
+  int data;
+  struct binary_tree_node_s *left, *right;
+} BTNode;
+
+typedef struct opt {
+  bool safe;
+  BTNode* ptr;
+} Opt;
+
+-- extern int hw();
+-- extern Opt hw2();
+extern Opt proc();
+
+end
+
+alloy c opaque_extern_type S => BTNode where
+  -- foreach(s, f) := lean_inc(f); lean_apply_1(f, s->m_s)
+  toLean => "CFoo_to_lean"
+  ofLean => "of_LeanFoo"
+  hw => "sad"
+  finalize(s) := free(s)
+
+alloy c section
+
+lean_object* traverse(BTNode* ptr) {
+  if (ptr == NULL) {
+    return lean_box(0);
+  } else {
+    lean_object * lo = lean_alloc_ctor(1, 3, 8 * 3);
+    lean_ctor_set(lo, 0, lean_box(ptr->data));
+    lean_ctor_set(lo, 1, traverse(ptr->left));
+    lean_ctor_set(lo, 2, traverse(ptr->right));
+    return lo;
+  }
+}
+
+end
+
+-- alloy c opaque_extern_type COpt => Opt where
+--   toLean => "COpt_to_lean"
+--   ofLean => "of_lean_COpt"
+--   is_safe(s) := if (s.safe) {
+--     return true
+--   } else {
+--     return false
+--   }
+--   finalize(s) := {}
+
+
+inductive Tree :=
+  | nil
+  | branch (d : Int) (l r : Tree)
+
+instance : Inhabited Tree := ⟨.nil⟩
+
+alloy c extern "ct" def ct (a : Unit) : Option Tree := {
+  printf("Entering ct\n");
+  Opt o = proc();
+  printf("Exited proc\n");
+  if (!o.safe) {
+    return lean_box(0);
+  } else {
+    lean_object * ob = lean_alloc_ctor(1, 1, 8);
+    lean_ctor_set(ob, 0, traverse(o.ptr));
+    return ob;
+  }
+}
