Main.lean
@@ -1,4 +1,23 @@
-import Backend
+import Backend.PythonAdapter
+
+@[match_pattern] def Tree.singleton (data : Int) : Tree := .branch data .nil .nil
+
+def Tree.toString : Tree -> String
+  | .nil => "·"
+  | .singleton data => s!"{data}"
+  | .branch data left right =>
+    let x := left.toString
+    let y := toString right
+    s!"{data}, \{{x}} \{{y}}"
+
+instance : ToString (Tree) := ⟨Tree.toString⟩
+
 
 def main : IO Unit :=
-  IO.println s!"Hello, {hello}!"
+  let x := ct ()
+  match x with
+  | .none => IO.println "Geh"
+  | .some t => IO.println s!"Hello¬{t}"
+
+
+-- #eval! (ct (1 : UInt32))
