lakefile.lean
@@ -1,7 +1,6 @@
 import Lake
 open Lake DSL
 
-
 package "Backend" where
   -- Settings applied to both builds and interactive editing
   leanOptions := #[
@@ -11,8 +10,87 @@ package "Backend" where
 
 require "leanprover-community" / "batteries" @ "git#v4.13.0"
 require alloy from git "https://github.com/tydeu/lean4-alloy.git"
+require Parser from git "https://github.com/fgdorais/lean4-parser"
 
+target pythonAdapter pkg : FilePath := do
+  let srcDir := pkg.dir / "Backend"
+  let outputFile := srcDir / "libpython_adapter.a"
+
+  -- Create a job to track the source file
+  -- let srcJob ← inputTextFile <| srcDir / "PythonAdapter.c"
+
+  -- Run the system make command instead of trying to compile directly with Lake
+  proc {
+    cmd := "make"
+    cwd := some srcDir
+  }
+
+  return BuildJob.pure outputFile
+
+
+-- extern_lib python_native pkg :=
+--    inputTextFile <| pkg.dir / python_include_dir / nameToStaticLib "python_native"
+
+module_data alloy.c.o.export : BuildJob System.FilePath
+module_data alloy.c.o.noexport : BuildJob System.FilePath
+
+lean_lib «Backend» where
+  precompileModules := true
+  -- supportInterpreter := true
+  nativeFacets := fun shouldExport =>
+    if shouldExport then
+      #[Module.oExportFacet, `alloy.c.o.export]
+    else
+      #[Module.oNoExportFacet, `alloy.c.o.noexport]
+  -- weakLeancArgs := #[
+  --   "-I", python_include_dir
+  -- ]
+  -- and whatever other configuration options you wish to add
+
+-- target ffi.o pkg : FilePath := do
+--   let oFile := pkg.buildDir / "c" / "ffi.o"
+--   let srcJob ← inputTextFile <| pkg.dir / "c" / "ffi.cpp"
+--   let weakArgs := #["-I", (← getLeanIncludeDir).toString]
+--   buildO oFile srcJob weakArgs #["-fPIC"] "c++" getLeanTrace
+
+-- extern_lib libleanffi pkg := do
+--   let ffiO ← ffi.o.fetch
+--   let name := nameToStaticLib "leanffi"
+--   buildStaticLib (pkg.nativeLibDir / name) #[ffiO]
+
+extern_lib extlib pkg := do
+
+  -- Create a job to track the source file
+  -- let srcJob ← inputTextFile <| srcDir / "PythonAdapter.c"
+
+  -- Run the system make command instead of trying to compile directly with Lake
+  proc {
+    cmd := "make"
+    cwd := some $ pkg.dir / "Backend"
+  }
+
+  println!(pkg.dir)
+  proc {
+    cmd := "ranlib"
+    args := #["libpython_adapter.a"]
+    cwd := some $ pkg.dir / "Backend"
+  }
+
+  return BuildJob.pure $ pkg.dir / "Backend" / "libpython_adapter.a"
+  -- println! "Hello"
+  -- ffiO
+  -- buildStaticLib (pkg.nativeLibDir / (nameToStaticLib "leanffi")) #[ffiO]
+
+extern_lib pythonItself := do
+  return BuildJob.pure $ "/opt/homebrew/opt/python@3.13/Frameworks/Python.framework/Versions/3.13/lib/libpython3.13.dylib"
 
 @[default_target]
-lean_lib «Backend» where
-  -- add any library configuration options here
+lean_exe «BackendExe» where
+  root := `Main
+  -- Enables the use of the Lean interpreter by the executable (e.g.,
+  -- `runFrontend`) at the expense of increased binary size on Linux.
+  -- Remove this line if you do not need such functionality.
+  supportInterpreter := true
+  -- weakLeancArgs := #[
+  --   "-I", python_include_dir
+  -- ]
