playground/expressionProblem.lean
@@ -1,0 +1,202 @@
+
+/-
+```python
+
+"(1 + 2) + (3 + 4)" --> parse this into the tree below
+
+(1 + 2) + 3
+
+
+     +
+   /   \
+  +      +
+ / \    / \
+1  2   3   4
+
+abstract class Tree {}
+class Empty extends Tree {}
+class Plus extends Tree {
+  Tree left, right;
+}
+
+     +
+   /   \
+  +     3
+ / \
+1  2
+
+class Tree
+class Leaf(Tree)
+  n : int
+
+@dataclass class Plus(Tree)
+  left : Tree
+  right : Tree
+
+
+Plus(Plus(Leaf(1), Leaf(2)), Leaf(3))
+
+
+
+
+
+"(1 + 1) * 3" --> parse it into some structured object
+     *
+   /   \
+  +     3
+ / \
+1  1
+
+class Tree(abc):
+  def calc(self): ...
+
+class Leaf(Tree):
+  n : int
+
+  def calc(self):
+    return self.n
+
+class Plus(Tree):
+  left : Tree
+  right : Tree
+  def __init__(self, left : Tree, right : Tree): ...
+
+  def calc(self):
+    return self.left.calc() + self.right.calc()
+
+class Mul(Tree):
+  left : Tree
+  right : Tree
+
+  def calc(self):
+    return self.left.calc() * self.right.calc()
+
+
+     +
+   /   \
+  *     3
+ / \
+1  1
+
+Plus(Mul(Leaf(1), Leaf(2)), Leaf(3)).calc()
+
+
+abstract class Arith {
+  ...
+}
+
+class Const extends Arith {
+  int n;
+  ...
+}
+
+class Add extends Arith {
+  Arith e1, e2;
+  ...
+
+}
+
+class Mult extends Arith {
+  Arith e1, e2;
+  ...
+
+}
+```
+
+-/
+
+
+
+
+/-
+def f ():
+  x = 3
+  y = 2 + x
+  return y + x
+
+def g (): return 5
+
+-/
+
+inductive Expression :=
+  | const (n : Nat)
+  | var (s : String)
+  | plus   : Expression -> Expression -> Expression
+  | mul    : Expression -> Expression -> Expression
+
+inductive PrimOp :=
+  | shape
+  | reshape
+  | stack
+  | matmul
+  | add
+  | mean
+  | softmax
+  | zeros
+  | ones
+  | tensor
+  | slicing
+
+inductive Statement :=
+  | assign (name : String) (expression : Expression)
+  | ret (expression : Expression)
+
+def Function := List Statement
+def Program := List Function
+
+example : Function := [
+  .assign "x" (.const 3),
+  .assign "y" (.plus (.const 2) (  ))
+]
+
+variable (Tensor : List Nat -> Type)
+
+example (a b : Tensor [1, 2, 3]) : Function (Tensor [1, 2, 3]) := [
+  .assign "x" (a + b),
+  ret (.var "x")
+]
+
+inductive Arith' :=
+  | Leaf (n : Nat)
+  | Plus : Arith' -> (Arith' -> Arith')
+  | Mul : Arith' -> (Arith' -> Arith')
+
+def add1 : Nat × Nat -> Nat := fun (a, b) => a + b
+def add2 : Nat -> (Nat -> Nat) := fun a => fun b => a + b
+/-
+
+def f (a) :
+  def g (b) :
+    return a + b
+  return g
+
+f (3)
+=
+def g (b) :
+  return 3 + b
+return g
+
+
+add2 (3)
+  ~> ( fun a => fun b => a + b ) (3)
+  ~> ( fun b => 3 + b )
+add2 (3) (4)
+  ~> ( (fun a => fun b => a + b) (3) ) (4)
+  ~> ( fun b => 3 + b ) (4)
+  3 + 4
+
+-/
+
+#reduce ((fun a => fun b => a + b) 3)
+
+
+#check ((3, 2) : Nat × Nat)
+
+def Arith.calc (self : Arith) : Nat :=
+  match self with
+  | Arith.Leaf n => n
+  | Arith.Plus (left, right) => left.calc + right.calc
+  | Arith.Mul  (left, right) => left.calc * right.calc
+
+#check (.Plus (.Mul (.Leaf 1, .Leaf 2), .Leaf 3) : Arith)
+#check (.Plus (.Mul (.Leaf 1, .Leaf 2), .Leaf 3) |> Arith.calc)
